Able to use global variables in etcd-raft proof

new/proof/go_etcd_io/raft/v3_proof/base.v
@@ -8,124 +8,127 @@ Section init.
 Context `{hG: heapGS Σ, !ffi_semantics _ _}.
 Context `{!globalsGS Σ} {go_ctx : GoContext}.
 
-Local Notation deps := (ltac2:(build_pkg_init_deps 'raftpb) : iProp Σ) (only parsing).
+Local Notation deps_raftpb := (ltac2:(build_pkg_init_deps 'raftpb) : iProp Σ) (only parsing).
 #[global] Program Instance : IsPkgInit raftpb :=
   {|
     is_pkg_init_def := True;
-    is_pkg_init_deps := deps;
+    is_pkg_init_deps := deps_raftpb;
   |}.
 
-Local Notation deps := (ltac2:(build_pkg_init_deps 'strconv) : iProp Σ) (only parsing).
+Local Notation deps_strconv := (ltac2:(build_pkg_init_deps 'strconv) : iProp Σ) (only parsing).
 #[global] Program Instance : IsPkgInit strconv :=
   {|
     is_pkg_init_def := True;
-    is_pkg_init_deps := deps;
+    is_pkg_init_deps := deps_strconv;
   |}.
 
-Local Notation deps := (ltac2:(build_pkg_init_deps 'slices) : iProp Σ) (only parsing).
+Local Notation deps_slices := (ltac2:(build_pkg_init_deps 'slices) : iProp Σ) (only parsing).
 #[global] Program Instance : IsPkgInit slices :=
   {|
     is_pkg_init_def := True;
-    is_pkg_init_deps := deps;
+    is_pkg_init_deps := deps_slices;
   |}.
 
-Local Notation deps := (ltac2:(build_pkg_init_deps 'strings) : iProp Σ) (only parsing).
+Local Notation deps_strings := (ltac2:(build_pkg_init_deps 'strings) : iProp Σ) (only parsing).
 #[global] Program Instance : IsPkgInit strings :=
   {|
     is_pkg_init_def := True;
-    is_pkg_init_deps := deps;
+    is_pkg_init_deps := deps_strings;
   |}.
 
-Local Notation deps := (ltac2:(build_pkg_init_deps 'math) : iProp Σ) (only parsing).
+Local Notation deps_math := (ltac2:(build_pkg_init_deps 'math) : iProp Σ) (only parsing).
 #[global] Program Instance : IsPkgInit math :=
   {|
     is_pkg_init_def := True;
-    is_pkg_init_deps := deps;
+    is_pkg_init_deps := deps_math;
   |}.
 
-Local Notation deps := (ltac2:(build_pkg_init_deps 'fmt) : iProp Σ) (only parsing).
+Local Notation deps_fmt := (ltac2:(build_pkg_init_deps 'fmt) : iProp Σ) (only parsing).
 #[global] Program Instance : IsPkgInit fmt :=
   {|
     is_pkg_init_def := True;
-    is_pkg_init_deps := deps;
+    is_pkg_init_deps := deps_fmt;
   |}.
 
-Local Notation deps := (ltac2:(build_pkg_init_deps 'quorum) : iProp Σ) (only parsing).
+Local Notation deps_quorum := (ltac2:(build_pkg_init_deps 'quorum) : iProp Σ) (only parsing).
 #[global] Program Instance : IsPkgInit quorum :=
   {|
     is_pkg_init_def := True;
-    is_pkg_init_deps := deps;
+    is_pkg_init_deps := deps_quorum;
   |}.
 
-Local Notation deps := (ltac2:(build_pkg_init_deps 'tracker) : iProp Σ) (only parsing).
+Local Notation deps_tracker := (ltac2:(build_pkg_init_deps 'tracker) : iProp Σ) (only parsing).
 #[global] Program Instance : IsPkgInit tracker :=
   {|
     is_pkg_init_def := True;
-    is_pkg_init_deps := deps;
+    is_pkg_init_deps := deps_tracker;
   |}.
 
-Local Notation deps := (ltac2:(build_pkg_init_deps 'confchange) : iProp Σ) (only parsing).
+Local Notation deps_confchange := (ltac2:(build_pkg_init_deps 'confchange) : iProp Σ) (only parsing).
 #[global] Program Instance : IsPkgInit confchange :=
   {|
     is_pkg_init_def := True;
-    is_pkg_init_deps := deps;
+    is_pkg_init_deps := deps_confchange;
   |}.
 
-Local Notation deps := (ltac2:(build_pkg_init_deps 'big) : iProp Σ) (only parsing).
+Local Notation deps_big := (ltac2:(build_pkg_init_deps 'big) : iProp Σ) (only parsing).
 #[global] Program Instance : IsPkgInit big :=
   {|
     is_pkg_init_def := True;
-    is_pkg_init_deps := deps;
+    is_pkg_init_deps := deps_big;
   |}.
 
-Local Notation deps := (ltac2:(build_pkg_init_deps 'rand) : iProp Σ) (only parsing).
+Local Notation deps_rand := (ltac2:(build_pkg_init_deps 'rand) : iProp Σ) (only parsing).
 #[global] Program Instance : IsPkgInit rand :=
   {|
     is_pkg_init_def := True;
-    is_pkg_init_deps := deps;
+    is_pkg_init_deps := deps_rand;
   |}.
 
-Local Notation deps := (ltac2:(build_pkg_init_deps 'bytes) : iProp Σ) (only parsing).
+Local Notation deps_bytes := (ltac2:(build_pkg_init_deps 'bytes) : iProp Σ) (only parsing).
 #[global] Program Instance : IsPkgInit bytes :=
   {|
     is_pkg_init_def := True;
-    is_pkg_init_deps := deps;
+    is_pkg_init_deps := deps_bytes;
   |}.
 
-Local Notation deps := (ltac2:(build_pkg_init_deps 'os) : iProp Σ) (only parsing).
+Local Notation deps_os := (ltac2:(build_pkg_init_deps 'os) : iProp Σ) (only parsing).
 #[global] Program Instance : IsPkgInit os :=
   {|
     is_pkg_init_def := True;
-    is_pkg_init_deps := deps;
+    is_pkg_init_deps := deps_os;
   |}.
 
-Local Notation deps := (ltac2:(build_pkg_init_deps 'log) : iProp Σ) (only parsing).
+Local Notation deps_log := (ltac2:(build_pkg_init_deps 'log) : iProp Σ) (only parsing).
 #[global] Program Instance : IsPkgInit log :=
   {|
     is_pkg_init_def := True;
-    is_pkg_init_deps := deps;
+    is_pkg_init_deps := deps_log;
   |}.
 
-Local Notation deps := (ltac2:(build_pkg_init_deps 'io) : iProp Σ) (only parsing).
+Local Notation deps_io := (ltac2:(build_pkg_init_deps 'io) : iProp Σ) (only parsing).
 #[global] Program Instance : IsPkgInit io :=
   {|
     is_pkg_init_def := True;
-    is_pkg_init_deps := deps;
+    is_pkg_init_deps := deps_io;
   |}.
 
-Local Notation deps := (ltac2:(build_pkg_init_deps 'errors) : iProp Σ) (only parsing).
+Local Notation deps_errors := (ltac2:(build_pkg_init_deps 'errors) : iProp Σ) (only parsing).
 #[global] Program Instance : IsPkgInit errors :=
   {|
     is_pkg_init_def := True;
-    is_pkg_init_deps := deps;
+    is_pkg_init_deps := deps_errors;
   |}.
 
-Definition foo := ltac2:(build_pkg_init ()).
+Definition is_initialized : iProp Σ :=
+  ∃ errStopped,
+    "ErrStopped" ∷ (global_addr raft.ErrStopped) ↦□ errStopped ∗
+    "%HErrStopped" ∷ ⌜ errStopped ≠ interface.nil ⌝.
 
 Local Notation deps := (ltac2:(build_pkg_init_deps 'raft) : iProp Σ) (only parsing).
 #[global] Program Instance : IsPkgInit raft :=
   {|
-    is_pkg_init_def := True;
+    is_pkg_init_def := is_initialized;
     is_pkg_init_deps := deps;
   |}.
 
