new/proof/go_etcd_io/raft/v3.v
@@ -1,6 +1,7 @@
 From New.code.go_etcd_io.raft Require Import v3.
 Require Import New.generatedproof.go_etcd_io.raft.v3
   New.generatedproof.go_etcd_io.raft.v3.raftpb.
+From New.proof.go_etcd_io.raft.v3_proof Require Export base protocol.
 From New.proof Require Import grove_prelude.
 
 Section proof.
